\section{Constrained Zonotopes}
\subsection{Basic Definition}
\begin{definition}
    $Z \subset \R^n$ is \emph{\textbf{Constrained Zonotope}} if \begin{equation}\label{eq:const_zonotope_def}
        \exists (\vb{G}, \vb{c}, \vb{A}, \vb{b}) 
            \in \R^{n \cross n_g} \cross \R^{n} \cross \R^{n_c \cross n_g} \cross \R^{n_c} 
        \st Z = \qty{
            \vb{G} \vb{\xi} + \vb{c} 
            \st \norm{\vb{\xi}}_\infty \leq 1 
                \land \vb{A} \vb{\xi} = \vb{b}
        }
    \end{equation}
\end{definition}

\textbf{Notes:}
\begin{itemize}
    \item $Z$ defined by \eqref{eq:const_zonotope_def} can be denoted by $Z = \{\vb{G}, \vb{c}, \vb{A}, \vb{b}\}$.
    \item $Z = \{\vb{G}, \vb{c}, \vb{A}, \vb{b}\}$ is known as a \emph{\textbf{constrained generator representation}} (CG-rep).
\end{itemize}

\textbf{Properties:}
\begin{enumerate}
    \item Constrained Zonotopes are affine image of a constrained unit hypercube $B_{\infty}(\vb{A},\vb{b}) \equiv \{\xi \in B_\infty \st \vb{A} \vb{\xi} \st \vb{A} \vb{\xi} = \vb{b}\}$.
\end{enumerate}

\subsection{Basic Operations:}
Let $Z = \{\vb{G}_z, \vb{c}_z, \vb{A}_z, \vb{b}_z\} \subset \R^n$, 
$W = \{\vb{G}_w, \vb{c}_w, \vb{A}_w, \vb{b}_q\} \subset \R^n$, 
$Y = \{\vb{G}_y, \vb{c}_y, \vb{A}_y, \vb{b}_y\} \subset \R^k$, 
and $\vb{R} \in \R^{k \cross n}$.

\textbf{Linear Mapping:}
\begin{equation}
    \vb{R} Z = \qty{
        \vb{R} \vb{G}_z, 
        \vb{R} \vb{c}_z, 
        \vb{A}_{z}, 
        \vb{b}_z
    }
\end{equation}

\textbf{Minkowski Sum:}
\begin{equation}
    Z + W    = \qty{
        \mqty[\vb{G}_z & \vb{G}_w], 
        \vb{c}_z + \vb{c}_w, 
        \mqty[
            \vb{A}_z & \vb{0}\\
            \vb{0}   &\vb{A}_w
        ],
        \mqty[
            \vb{b}_z\\
            \vb{b}_w
        ]
    }
\end{equation}

\textbf{Generalized Intersection:}
\begin{equation}
    Z \cap_{\vb{R}} Y = \qty{
        \mqty[\vb{G}_z & \vb{0}],
        \vb{c}_z,
        \mqty[
            \vb{A}_z &\vb{0}\\
            \vb{0} &\vb{A}_y\\
            \vb{R} \vb{G}_z &-\vb{G}_y
        ],
        \mqty[
            \vb{b}_z\\
            \vb{b}_y\\
            \vb{c}_y - \vb{R} \vb{c}_z
        ]
    }
\end{equation}

\subsection{Relationship to Convex Polytope}
$Z \subset \R^n$ is a constrained zonotope iff it is a convex polytope.
(i.e.) $\forall_{Z \subset \R^n}$ \[
     Z \text{ constrained polytope } \iff Z \text{ convex polytope}
\] or equivalently $\forall_{Z = P \subset \R^n}$ \[
    \exists \qty(\vb{G}, \vb{c}, \vb{A}, \vb{b}) \st Z = \{\vb{G}, \vb{c}, \vb{A}, \vb{b}\}
    \iff \exists \qty(\vb{H}, \vb{k}) \st P = \{\vb{H}, \vb{k}\}
\]

\subsection{Complexity Reduction}
\subsubsection{Rescaling Constrained Zonotopes}
Let $Z = \{\vb{G}, \vb{c}, \vb{A}, \vb{b}\}$.
For $\xi^{L}, \xi^{U} \in \R^n \st B_\infty(\vb{A},\vb{b}) \subset [\xi^{L},\xi^{U}] \subset [-\vb{1}, \vb{1}]$, there is an equivelent CG-rep as \begin{equation}
    Z = \qty{
        \vb{G} \text{diag}(\vb{\xi}_r), 
        \vb{c} + \vb{G} \vb{\xi}_m,
        \vb{A} \text{diag}(\vb{\xi}_r),
        \vb{b} - \vb{A} \vb{\xi}_m
    }
\end{equation}
with $\vb{\xi}_m = \frac{1}{2} (\vb{\xi}^{U} + \vb{\xi}^{L})$ and $\vb{\xi}_r = \frac{1}{2} (\vb{\xi}^{U} - \vb{\xi}^{L})$.

\textbf{Notes:}
\begin{itemize}
    \item Best interval is just solving for an LP ($\min$ or $\max$ satisfying the equivelency and $\infty$-norm ball ineqality) but it's cheaper to do a different method...
\end{itemize}


\subsubsection{Constraint Reduction}
Let $Z = \{\vb{G}, \vb{c}, \vb{A}, \vb{b}\}$.
A reduced constraint set $\tilde{Z}$ with $Z \subset \tilde{Z}$ exists $\forall \Lambda_G \in \R^{n \cross n_c}, \Lambda_A \in \R^{n_c \cross n_c}$ defined by \begin{equation}
    \tilde{Z} = \qty{
        \vb{G} - \Lambda_G \vb{A}, 
        \vb{c} + \Lambda_G \vb{b},
        \vb{A} - \Lambda_A \vb{A},
        \vb{b} - \Lambda_A \vb{b}
    }
\end{equation}

\textbf{Eliminate single constraints}
A single constraint equation is given by \begin{equation}
    \xi_j = a_{1j}^{-1} b_j - a_{1j}^{-1} \sum_{k \neq j} a_{1k} \xi_k
\end{equation} with the entire form as \[
    \vb{z} = \vb{G} \vb{\xi} + \vb{c}
\]

To eliminate the $j$-th constraint we construct $\Lambda_G$ and $\lambda_A$ as \begin{equation}
    \Lambda_G \equiv \vb{G} \vb{E}_{j1} a_{1j}^{-1}, 
    \quad
    \Lambda_A \equiv \vb{A} \vb{E}_{j1} a_{1j}^{-1}
\end{equation}
using $\vb{E}_{j1} \in \R^{n_g \cross n_c}$ with all zero except for a 1 in $(j,1)$.

This results in \[
    \tilde{Z} = \qty{
        \vb{G} - \Lambda_G \vb{A}, 
        \vb{c} + \Lambda_G \vb{b},
        \vb{A} - \Lambda_A \vb{A},
        \vb{b} - \Lambda_A \vb{b}
    } = \qty{
        \tilde{\vb{G}},
        \tilde{\vb{c}},
        \tilde{\vb{A}},
        \tilde{\vb{b}}
    }
\]


We can eliminate the 


